[SI] specs using local (cache) points-to connective.

aneris/examples/snapshot_isolation/specs/events.v
@@ -1,23 +1,30 @@
+
 From aneris.aneris_lang Require Import lang.
 From aneris.examples.snapshot_isolation.specs
      Require Import user_params  time.
 
 (** Write and apply events *)
 
-Section Write_event.
+Section Events.
   Context `{!KVS_time}.
 
-  Definition EV_id : Set := socket_address * nat.
+  (* Definition EV_id : Set := socket_address * nat. *)
 
  (** Write event *)
-  Record we :=
+  Record write_event :=
     {
       we_key : Key;
       we_val : val;
       we_time : Time;
     }.
+ (** Cache event *)
+  Record cache_event :=
+   {
+     cache_snap : option write_event;
+     cache_newv : option val;
+    }.
 
-End Write_event.
+End Events.
 
 Notation "s '<ₜ' t" :=
   (TM_lt (we_time s) (we_time t)) (at level 70, no associativity).
@@ -31,10 +38,10 @@ Notation "s '=ₜ' t" :=
 Section Events_lemmas.
   Context `{!KVS_time}.
 
-  Global Instance we_dec : EqDecision we.
+  Global Instance write_event_dec : EqDecision write_event.
   Proof. solve_decision. Qed.
 
-  Global Instance we_countable : Countable we.
+  Global Instance write_event_countable : Countable write_event.
   Proof.
     refine {| encode := λ a, encode (we_key a, we_val a, we_time a);
               decode := λ n,
@@ -42,6 +49,21 @@ Section Events_lemmas.
                                we_time := x.2; |}) <$>
                         @decode
                         (Key * val * Time)%type
+                        _ _ n
+           |}.
+    by intros []; rewrite /= decode_encode /=.
+  Qed.
+
+  Global Instance cahce_event_dec : EqDecision cache_event.
+  Proof. solve_decision. Qed.
+
+  Global Instance cache_event_countable : Countable cache_event.
+  Proof.
+    refine {| encode := λ a, encode (cache_snap a, cache_newv a);
+              decode := λ n,
+                      (λ x, {| cache_snap := x.1; cache_newv := x.2; |}) <$>
+                        @decode
+                        (option write_event * option val)%type
                         _ _ n
            |}.
     by intros []; rewrite /= decode_encode /=.
