aneris/examples/snapshot_isolation/specs/specs.v
@@ -11,126 +11,140 @@ From aneris.examples.snapshot_isolation
 From aneris.examples.snapshot_isolation.specs
      Require Import user_params time events resources.
 
+Definition cache_commit `{!KVS_time}  c k t : option write_event :=
+    match c.(cache_newv) with
+      | None => c.(cache_snap)
+      | Some v => Some {| we_key := k;  we_val := v; we_time := t; |}
+    end.
+
+Definition max_timestamp `{!KVS_time} t (m : gmap Key (option write_event)) : Prop :=
+    ∀ k (e : write_event), m !! k = Some (Some e) → TM_lt e.(we_time) t.
+
+Definition can_commit `{!KVS_time}
+    (m : gmap Key (option write_event))
+    (mc : gmap Key cache_event) : Prop :=
+    ∀ (k : Key) (ce : cache_event),
+       k ∈ dom m → (mc !! k) = Some ce → is_Some (ce.(cache_newv)) →
+       m !! k = Some ce.(cache_snap).
+
+Definition cache_updv `{!KVS_time} (c : cache_event) (v : val) : cache_event :=
+  {|cache_snap := c.(cache_snap); cache_newv := Some v |}.
+
+Definition cache_getv `{!KVS_time} (c : cache_event) : option val :=
+  match c.(cache_newv) with
+  | Some v => Some v
+  | None =>
+      match c.(cache_snap) with
+      | Some we => Some we.(we_val)
+      | None => None
+      end
+  end.
+
+Definition cache_make `{!KVS_time} (we : option write_event) : cache_event :=
+  {|cache_snap := we; cache_newv := None |}.
+
+Definition kvs_snap_coh `{!KVS_time}
+  (ms m : gmap Key (option write_event)) : Prop :=
+  dom m = dom ms ∧
+    ∀ k we, k ∈ dom ms →
+       ms !! k = Some (Some we) →
+      ∃ we', m !! k = Some (Some we') ∧ we ≤ₜ we'.
+
+Definition snap_cache_coh `{!KVS_time}
+  (ms : gmap Key (option write_event)) (mc : gmap Key cache_event) : Prop :=
+  dom ms = dom mc ∧
+    ∀ k (wo : option write_event), k ∈ dom ms →
+       ms !! k = Some wo →
+      ∃ c, mc !! k = Some c ∧ c.(cache_snap) = wo.
+
 
 (** Specifications for read and write operations.  *)
 Section Specification.
   Context `{!anerisG Mdl Σ, !User_params, !KVS_time,
             !KVS_snapshot_isolation_api, !SI_resources Mdl Σ}.
 
-  Definition write_spec : Prop :=
+
+  Definition write_spec : iProp Σ :=
     ∀ (cstate : val) (sa : socket_address)
-      (ms : gmap Key (option we))
-      (mc : gmap Key val) E
-      (k : Key) (v : SerializableVal),
+      (c : cache_event)
+      (k : Key) (v : SerializableVal) E,
     ⌜k ∈ KVS_keys⌝ -∗
-    {{{ ConnectionState cstate (Active ms mc) }}}
+    {{{ k ↦ₜ c }}}
       SI_write cstate #k v @[ip_of_address sa] E
-    {{{ RET #();
-        ConnectionState cstate (Active ms (<[k:= v.(SV_val)]> mc)) }}}.
+    {{{ RET #(); k ↦ₜ cache_updv c v }}}.
 
-  Definition read_spec : Prop :=
+  Definition read_spec : iProp Σ :=
     ∀ (cstate : val) (sa : socket_address)
-      (ms : gmap Key (option we))
-      (mc : gmap Key val)
-      (eo : option we) E
-     (k : Key), ⌜ms !! k = Some eo⌝ -∗
-    {{{ ConnectionState cstate (Active ms mc) }}}
+      (k : Key) (c : cache_event) E,
+    {{{ k ↦ₜ c }}}
       SI_read cstate #k @[ip_of_address sa] E
-    {{{ (ro : val), RET $ro; ConnectionState cstate (Active ms mc) ∗
-        ⌜(k ∉ dom mc ∧
-        match eo with
-           | (Some we) => ro = SOMEV we.(we_val)
-           | None => ro = NONEV
-         end) ∨
-        ∃ v, Some v = (mc !! k) ∧ ro = $(Some v)⌝ }}}.
+    {{{ vo, RET vo; ⌜vo = $(cache_getv c)⌝ ∗ k ↦ₜ c }}}.
 
-  Definition start_spec : Prop :=
+  Definition start_spec : iProp Σ :=
     ∀ (cstate : val) (sa : socket_address)
        (E : coPset),
     ⌜↑KVS_InvName ⊆ E⌝ -∗
-    <<< ∀∀ (m : gmap Key (option we)),
+    <<< ∀∀ (m : gmap Key (option write_event)),
        ConnectionState cstate CanStart ∗
        [∗ map] k ↦ eo ∈ m, k ↦ₖ eo >>>
       SI_start cstate @[ip_of_address sa] E
     <<<▷ RET #();
-       ConnectionState cstate (Active m ∅) ∗
-       [∗ map] k ↦ eo ∈ m, k ↦ₖ eo >>>.
+       ConnectionState cstate (Active m) ∗
+       ([∗ map] k ↦ eo ∈ m, k ↦ₖ eo) ∗
+       ([∗ map] k ↦ eo ∈ m, k ↦ₜ cache_make eo) >>>.
 
-  Definition can_commit
-    (m ms : gmap Key (option we))
-    (mc : gmap Key val) : Prop :=
-    ∀ k, is_Some (mc !! k) → ms !! k = m !! k.
-
-  Definition max_timestamp t (m : gmap Key (option we)) : Prop :=
-    ∀ k (e : we), m !! k = Some (Some e) → TM_lt e.(we_time) t.
-
-  Definition commit_spec : Prop :=
+  Definition commit_spec : iProp Σ :=
    ∀ (cstate : val) (sa : socket_address)
-     (P :  gmap Key (option we) → iProp Σ)
-     (Q :  gmap Key (option we) → gmap Key val → iProp Σ)
+     (P :  gmap Key (option write_event) → iProp Σ)
+     (Q :  gmap Key (option write_event) → gmap Key cache_event → iProp Σ)
      (E : coPset),
     ⌜↑KVS_InvName ⊆ E⌝ -∗
-    <<< ∀∀ (m ms: gmap Key (option we)) (mc : gmap Key val),
-        ConnectionState cstate (Active ms mc) ∗
-        [∗ map] k ↦ eo ∈ m, k ↦ₖ eo ∗ P ms >>>
+    <<< ∀∀ (m ms: gmap Key (option write_event))
+           (mc : gmap Key cache_event),
+        ConnectionState cstate (Active ms) ∗
+        ⌜snap_cache_coh m mc⌝ ∗
+        ([∗ map] k ↦ eo ∈ m, k ↦ₖ eo) ∗
+        ([∗ map] k ↦ c ∈ mc, k ↦ₜ c) ∗
+        P ms >>>
       SI_commit cstate @[ip_of_address sa] E
     <<<▷∃∃ b, RET #b;
         ConnectionState cstate CanStart ∗
+         ⌜kvs_snap_coh ms m⌝ ∗
         (** Transaction has been commited. *)
-        (⌜b = true⌝ ∗ ⌜can_commit m ms mc⌝ ∗
-          ∃ (t: Time),
-            (** Pointers that have been only read *)
-           ([∗ set] k ∈ (dom m) ∖ (dom mc),
-              let weo :=
-              match (m !! k) with
-                | None => None
-                | Some weo => weo
-              end in k ↦ₖ weo) ∗
-            (** Pointers that have been written to *)
-            ([∗ map] k↦v ∈ mc,
-               k ↦ₖ Some {| we_key := k; we_val := v; we_time := t |}) ∗
-             ⌜max_timestamp t m⌝ ∗ Q ms mc) ∨
+        (⌜b = true⌝ ∗ ⌜can_commit m mc⌝ ∗
+          ∃ (t: Time), ⌜max_timestamp t m⌝ ∗
+            ([∗ map] k↦c ∈ mc,  k ↦ₖ cache_commit c k t) ∗ Q ms mc) ∨
         (** Transaction has been aborted. *)
-         (⌜b = false⌝ ∗ ⌜¬ can_commit m ms mc⌝ ∗
+         (⌜b = false⌝ ∗ ⌜¬ can_commit m mc⌝ ∗
            [∗ map] k ↦ eo ∈ m, k ↦ₖ eo) >>>.
 
-Definition run_spec : Prop :=
+Definition run_spec : iProp Σ :=
     ∀ (cstate : val) (tbody : val)
       (sa : socket_address) (E : coPset)
-      (ms : gmap Key (option we)) (mc : gmap Key val)
-      (P :  gmap Key (option we) → iProp Σ)
-      (Q :  gmap Key (option we) → gmap Key val → iProp Σ),
-    ⌜↑KVS_InvName ⊆ E⌝
-    -∗
-    {{{ ConnectionState cstate (Active ms ∅) ∗ P ms }}}
-      tbody cstate #() @[ip_of_address sa] E
-    {{{ RET #(); ConnectionState cstate (Active ms mc) ∗ Q ms mc }}}
+      (P :  gmap Key (option write_event) → iProp Σ)
+      (Q :  gmap Key (option write_event) → gmap Key cache_event → iProp Σ),
+    ⌜↑KVS_InvName ⊆ E⌝ -∗
+      (∀ (m0 : gmap Key (option write_event)) (mc : gmap Key cache_event),
+         {{{ ([∗ map] k ↦ wo ∈ m0, k ↦ₜ cache_make wo) ∗ P m0 }}}
+           tbody cstate #() @[ip_of_address sa] E
+         {{{ RET #(); ([∗ map] k ↦ c ∈ mc, k ↦ₜ c) ∗ Q m0 mc }}})
     →
-    <<< ∀∀ m,
-        ConnectionState cstate CanStart ∗ P ms ∗
-          [∗ map] k ↦ eo ∈ m, k ↦ₖ eo >>>
+    <<< ∀∀ m0, ConnectionState cstate CanStart ∗
+               P m0 ∗
+               [∗ map] k ↦ eo ∈ m0, k ↦ₖ eo >>>
            SI_run cstate tbody @[ip_of_address sa] E
-    <<<▷∃∃ b,  RET #b;
-        ConnectionState cstate CanStart ∗
-        (** Transaction has been commited. *)
-        (⌜b = true⌝ ∗ ⌜can_commit m ms mc⌝ ∗
-          ∃ (t: Time),
-            (** Pointers that have been only read *)
-           ([∗ set] k ∈ (dom m) ∖ (dom mc),
-              let weo :=
-              match (m !! k) with
-                | None => None
-                | Some weo => weo
-              end in k ↦ₖ weo) ∗
-            (** Pointers that have been written to *)
-            ([∗ map] k↦v ∈ mc,
-               k ↦ₖ Some {| we_key := k; we_val := v; we_time := t |}) ∗
-             ⌜max_timestamp t m⌝ ∗ Q ms mc) ∨
-        (** Transaction has been aborted. *)
-         (⌜b = false⌝ ∗ ⌜¬ can_commit m ms mc⌝ ∗
-           [∗ map] k ↦ eo ∈ m, k ↦ₖ eo) >>>.
+    <<<▷∃∃ m1 mc b, RET #b;
+               ConnectionState cstate CanStart ∗
+               ⌜kvs_snap_coh m0 m1⌝ ∗
+               (** Transaction has been commited. *)
+               (⌜b = true⌝ ∗ ⌜can_commit m1 mc⌝ ∗
+                ∃ (t: Time), ⌜max_timestamp t m1⌝ ∗
+                  ([∗ map] k↦c ∈ mc,  k ↦ₖ cache_commit c k t) ∗ Q m0 mc) ∨
+               (** Transaction has been aborted. *)
+               (⌜b = false⌝ ∗ ⌜¬ can_commit m1 mc⌝ ∗
+                [∗ map] k ↦ eo ∈ m1, k ↦ₖ eo) >>>.
 
-  Definition init_client_proxy_spec : Prop :=
+  Definition init_client_proxy_spec : iProp Σ :=
     ∀ (sa : socket_address),
     {{{ unallocated {[sa]} ∗
         KVS_address ⤇ KVS_si ∗
@@ -140,7 +154,7 @@ Definition run_spec : Prop :=
                   #sa #KVS_address @[ip_of_address sa]
     {{{ cstate, RET cstate; ConnectionState cstate CanStart }}}.
 
-Definition init_kvs_spec : Prop :=
+Definition init_kvs_spec : iProp Σ :=
   {{{ KVS_address ⤇ KVS_si ∗
         KVS_address ⤳ (∅,∅) ∗
         free_ports (ip_of_address KVS_address)
@@ -173,41 +187,12 @@ Section SI_Module.
         True ⊢ |={E}=> ∃ (SIRes : SI_resources Mdl Σ),
        GlobalInv ∗
        ([∗ set] k ∈ KVS_keys, k ↦ₖ None) ∗
-       ⌜init_kvs_spec⌝ ∗
-       ⌜init_client_proxy_spec⌝ ∗
-       ⌜read_spec⌝ ∗
-       ⌜write_spec⌝ ∗
-       ⌜start_spec⌝ ∗
-       ⌜commit_spec⌝ ∗
-       ⌜run_spec⌝ }.
+       init_kvs_spec ∗
+       init_client_proxy_spec ∗
+       read_spec ∗
+       write_spec ∗
+       start_spec ∗
+       commit_spec ∗
+       run_spec }.
 
 End SI_Module.
-
-(* TODO: REMOVE THIS LATER, it's just an example of usage. *)
-Section Prove_of_t_body_of_some_example.
-  Context `{!anerisG Mdl Σ}.
-  Context `{!User_params, !KVS_time, !KVS_snapshot_isolation_api, !SI_resources Mdl Σ}.
-  Context (rd_spec : read_spec).
-
-  Definition code_snippet : val :=
-    λ: "cstate" "k", SI_read "cstate" "k".
-
-  Lemma code_snippet_proof sa (cstate : val) ms m (k : Key) :
-     {{{ ⌜k ∈ dom ms⌝ ∗
-           ConnectionState cstate (Active ms (<[k:=#42]> m))}}}
-       code_snippet cstate #k @[ip_of_address sa]
-     {{{ vo, RET vo; ⌜vo = $(Some 42)⌝ }}}.
- Proof.
-   rewrite /code_snippet.
-   iIntros (Φ) "(%Hkey & HConnectionState) HΦ".
-   wp_pures.
-   iApply (rd_spec with "[][$HConnectionState]").
-   - iPureIntro. admit.
-   - iNext.
-   iIntros (vo) "(_ & [%Habs | %Hpost])"; iApply "HΦ".
-   -- admit.
-   -- destruct Hpost as (v & Hv & Hvo).
-      by simplify_map_eq /=.
- Admitted.
-
-End Prove_of_t_body_of_some_example.
